add LowerBound.v

x86/AsmC.v
@@ -3,12 +3,10 @@ Require Import ASTC Integers Floats Values MemoryC Events Globalenvs Smallstep.
 Require Import Locations Stacklayout Conventions.
 (** newly added **)
 Require Export Asm.
-Require Import Simulation AsmregsC.
-Require Import Skeleton ModSem Mod.
+Require Import Simulation Asm ValuesC.
+Require Import Skeleton ModSem Mod sflib.
 
 Set Implicit Arguments.
-
-
 
 Definition get_mem (st: state): mem :=
   match st with
@@ -32,6 +30,31 @@ Definition st_m (st0: state): mem :=
   | State _ m => m
   end
 .
+
+Inductive store_arguments (m0: mem) (rs: regset) (vs: list val) (sg: signature) (m2: mem): Prop :=
+| store_arguments_intro
+    m1 blk
+    (ALC: Mem.alloc m0 0 (4 * size_arguments sg) = (m1, blk))
+    (VALS: extcall_arguments rs m2 sg vs)
+    (RSRSP: rs#RSP = Vptr blk Ptrofs.zero true)
+    (UNCH: Mem.unchanged_on
+             (fun b ofs' =>
+                if eq_block b blk
+                then ~ (0 <= ofs' <  4 * size_arguments sg)
+                else True) m1 m2)
+    (NB: m1.(Mem.nextblock) = m2.(Mem.nextblock))
+    (PERM: Mem.range_perm m2 blk 0 (4 * size_arguments sg) Cur Freeable)
+.
+
+Definition external_state F V (ge: Genv.t F V) (v : val) : bool :=
+  match v with
+  | Vptr blk ofs true =>
+    match (Genv.find_funct ge (Vptr blk Ptrofs.zero true)) with
+    | None => true
+    | _ => false
+    end
+  | _ => true
+  end.
 
 Section ASMEXTRA.
 
@@ -69,25 +92,6 @@ Section ASMEXTRA.
 End ASMEXTRA.
 (*** !!!!!!!!!!!!!!! REMOVE ABOVE AFTER MERGING WITH MIXED SIM BRANCH !!!!!!!!!!!!!!!!!! ***)
 
-
-
-
-
-
-
-
-
-
-
-
-
-
-
-
-
-
-
-
 Section MODSEM.
 
   Variable skenv_link: SkEnv.t.
@@ -97,34 +101,60 @@ Section MODSEM.
 
   Record state := mkstate {
     init_rs: regset;
-    st: Asm.state;
+    st:> Asm.state;
+    (* extret: bool; *)
   }.
 
-  Inductive at_external (skenv_link: SkEnv.t): state -> Args.t -> Prop :=
+  Inductive step (ge: genv) (st0: state) (tr: trace) (st1: state): Prop :=
+  | step_intro
+      (STEP: Asm.step ge st0.(st) tr st1.(st))
+      (INITRS: st0.(init_rs) = st1.(init_rs))
+      (* (ISRETURN: step_ret st0.(st) = st1.(extret)) *)
+  .
+
+  Record wf_RA (ra : val) : Prop :=
+    mk_wf_RA {
+        TPTR: Val.has_type ra Tptr;
+        RAFAKE: ~ is_real_ptr ra;
+        RADEF: ra <> Vundef;
+      }.
+
+  Inductive at_external: state -> Args.t -> Prop :=
   | at_external_intro
-      rs m0 m1 fptr sg vs blk ofs
-      (FPTR: rs # PC = fptr)
-      (EXTERNAL: Genv.find_funct ge fptr = None)
-      (SIG: exists skd, skenv_link.(Genv.find_funct) fptr = Some skd /\ SkEnv.get_sig skd = sg)
+      rs m0 m1 sg vs blk0 blk1 ofs
+      (FPTR: rs # PC = Vptr blk0 Ptrofs.zero true) (* TODO simplify it *)
+      (EXTERNAL: Genv.find_funct ge (Vptr blk0 Ptrofs.zero true) = None)
+      (SIG: exists skd, skenv_link.(Genv.find_funct) (Vptr blk0 Ptrofs.zero true)
+                        = Some skd /\ SkEnv.get_sig skd = sg)
       (VALS: extcall_arguments rs m0 sg vs)
-      (RSP: rs RSP = Vptr blk ofs true)
-      (FREE: Mem.free m0 blk ofs.(Ptrofs.unsigned) (1 + ofs.(Ptrofs.unsigned) + (size_arguments sg)) = Some m1)
+      (RSP: rs RSP = Vptr blk1 ofs true)
+      (RAPTR: <<TPTR: Val.has_type (rs RA) Tptr>> /\ <<RADEF: rs RA <> Vundef>>)
+      (OFSZERO: ofs = Ptrofs.zero)
+      (FREE: Mem.free m0 blk1 ofs.(Ptrofs.unsigned) (ofs.(Ptrofs.unsigned) + 4 * (size_arguments sg)) = Some m1)
       init_rs
     :
-      at_external skenv_link (mkstate init_rs (State rs m0)) (Args.mk fptr vs m1)
+      at_external (mkstate init_rs (State rs m0))
+                  (Args.mk (Vptr blk0 Ptrofs.zero true) vs m1)
   .
 
   Inductive initial_frame (args: Args.t)
     : state -> Prop :=
   | initial_frame_intro
-      fd m0 m1 rs blk
+      fd m rs sg
+      (SIG: sg = fd.(fn_sig))
       (FINDF: Genv.find_funct ge args.(Args.fptr) = Some (Internal fd))
-      (ALLOC: Mem.alloc args.(Args.m) 0 (size_arguments fd.(fn_sig)) = (m0, blk))
-      (PC: rs # PC = args.(Args.fptr))
-      (RPS: rs # RSP = Vptr blk Ptrofs.zero true)
-      (VALS: extcall_arguments rs m1 fd.(fn_sig) args.(Args.vs))
+      (RSPC: rs # PC = args.(Args.fptr))
+      (SZ: 4 * size_arguments sg <= Ptrofs.modulus)
+      (STORE: store_arguments args.(Args.m) rs args.(Args.vs) sg m)
+      (RAPTR: wf_RA (rs RA))
+      (PTRFREE: forall
+          pr mr
+          (MR: to_mreg pr = Some mr)
+          (NOTIN: ~In (R mr) (regs_of_rpairs (loc_arguments sg)))
+        ,
+          <<PTRFREE: ~ is_real_ptr (rs pr)>>)
     :
-      initial_frame args (mkstate rs (State rs m1))
+      initial_frame args (mkstate rs (State rs m))
   .
 
   Inductive final_frame: state -> Retv.t -> Prop :=
@@ -133,9 +163,15 @@ Section MODSEM.
       (CALLEESAVE: forall mr, Conventions1.is_callee_save mr ->
                               Val.lessdef (init_rs mr.(to_preg)) (rs mr.(to_preg)))
       (INITRSP: init_rs # RSP = Vptr blk Ptrofs.zero true)
-      (INITSIG: exists skd, skenv_link.(Genv.find_funct) (init_rs # PC) = Some skd /\ SkEnv.get_sig skd = sg)
-      (FREE: Mem.free m0 blk 0 (size_arguments sg) = Some m1)
+      (INITSIG: exists skd, skenv_link.(Genv.find_funct) (init_rs # PC)
+                            = Some skd /\ SkEnv.get_sig skd = sg)
+      (FREE: Mem.free m0 blk 0 (4 * size_arguments sg) = Some m1)
       (RETV: loc_result sg = One mr)
+      (EXTERNAL: external_state ge (rs # PC))
+      (RSRA: rs # PC = init_rs # RA)
+      (RAPTR: wf_RA (init_rs RA))
+      (* (RSRSP: Val.lessdef (rs # RSP) (init_rs # RSP)) *)
+      (RSRSP: rs # RSP = init_rs # RSP)
     :
       final_frame (mkstate init_rs (State rs m0)) (Retv.mk (rs mr.(to_preg)) m1)
   .
@@ -144,20 +180,15 @@ Section MODSEM.
   | after_external_intro
       init_rs rs0 m0 rs1 m1 retv
       sg blk ofs
-      (SIG: exists skd, skenv_link.(Genv.find_funct) (rs0 # PC) = Some skd /\ SkEnv.get_sig skd = sg)
-      (RS: rs1 = (set_pair (loc_external_result sg) retv.(Retv.v) (Asmregs.regset_after_external rs0)))
-      (RSP: rs0 RSP = Vptr blk ofs true)
-      (UNFREE: Mem_unfree m0 blk ofs.(Ptrofs.unsigned) (1 + ofs.(Ptrofs.unsigned) + (size_arguments sg)) = Some m1)
+      (SIG: exists skd, skenv_link.(Genv.find_funct) (rs0 # PC)
+                        = Some skd /\ SkEnv.get_sig skd = sg)
+      (RS: rs1 = (set_pair (loc_external_result sg) retv.(Retv.v) (regset_after_external rs0)) #PC <- (rs0 RA))
+      (RSRSP: rs0 RSP = Vptr blk ofs true)
+      (UNFREE: Mem_unfree retv.(Retv.m) blk ofs.(Ptrofs.unsigned) (ofs.(Ptrofs.unsigned) + 4 * (size_arguments sg)) = Some m1)
     :
       after_external (mkstate init_rs (State rs0 m0))
                      retv
                      (mkstate init_rs (State rs1 m1))
-  .
-
-  Inductive step (ge: genv) (st0: state) (tr: trace) (st1: state): Prop :=
-  | step_intro
-      (STEP: Asm.step ge st0.(st) tr st1.(st))
-      (INITRS: st0.(init_rs) = st1.(init_rs))
   .
 
   Program Definition modsem: ModSem.t :=
@@ -173,7 +204,7 @@ Section MODSEM.
   .
   Next Obligation.
     ii; ss; des. inv_all_once; des; ss; clarify. rewrite RSP in *. clarify.
-    determ_tac extcall_arguments_determ.
+    rewrite FPTR in *. clarify. f_equal. eapply extcall_arguments_determ; eauto.
   Qed.
   Next Obligation.
     ii; ss; des. inv_all_once; des; ss; clarify.
@@ -181,20 +212,21 @@ Section MODSEM.
     f_equal. rewrite RETV in *. clarify.
   Qed.
   Next Obligation.
-    ii; ss; des. inv_all_once; des; ss; clarify.
-    rewrite RSP in *. clarify.
+    ii; ss; des. inv_all_once; des; ss; clarify. f_equal.
+    rewrite RSRSP in *. clarify.
   Qed.
   Next Obligation.
     ii; ss; des. inv_all_once; des; ss; clarify.
-    admit "".
+    exfalso. inv STEP; ss; rewrite FPTR in *; inv H2; des_ifs.
+  Qed.
+  Next Obligation.
+    ii; ss; des. inv_all_once; ss; clarify. inv EXTERNAL.
+    unfold external_state in *.
+    des_ifs; inv STEP; ss; des_ifs; rewrite Heq in *; clarify.
   Qed.
   Next Obligation.
     ii; ss; des. inv_all_once; ss; clarify.
-    admit "".
-  Qed.
-  Next Obligation.
-    ii; ss; des. inv_all_once; ss; clarify.
-    admit "".
+    inv RAPTR0. rewrite FPTR in *. rewrite <- RSRA in *. ss.
   Qed.
 
   Lemma not_external
@@ -210,6 +242,7 @@ Section MODSEM.
 
   Lemma lift_receptive_at
         st
+        (* b *)
         (RECEP: receptive_at (semantics_with_ge ge) st)
     :
       forall init_rs, receptive_at modsem (mkstate init_rs st)
@@ -219,7 +252,7 @@ Section MODSEM.
     - inv H. ss. exploit sr_receptive_at; eauto.
       { eapply match_traces_preserved; try eassumption. ii; ss. }
       i; des.
-      eexists (mkstate _ s2). ss.
+      eexists (mkstate _ s2). econs; ss.
     - inv H. ss. exploit sr_traces_at; eauto.
   Unshelve.
     all: ss.
@@ -243,7 +276,7 @@ Section MODSEM.
     - inv H. inv H0. ss.
       determ_tac sd_determ_at. esplits; eauto.
       { eapply match_traces_preserved; try eassumption. ii; ss. }
-      i. clarify. destruct s1, s2; ss. f_equal; ss. eauto.
+      i. clarify. destruct s1, s2; ss. f_equal; ss; eauto.
     - inv H. ss. exploit sd_traces_at; eauto.
   Unshelve.
     all: ss.
@@ -258,10 +291,6 @@ Section MODSEM.
 
 
 End MODSEM.
-
-
-
-
 
 Section MODULE.
 
@@ -280,4 +309,3 @@ Section MODULE.
   Qed.
 
 End MODULE.
-
