x86/AsmgenproofC.v
@@ -3,30 +3,332 @@ Require Import Integers Floats AST Linking.
 Require Import Values Memory Events Globalenvs Smallstep.
 Require Import Op Locations MachC Conventions AsmC.
 Require Import Asmgen Asmgenproof0 Asmgenproof1.
-Require Import Asmregs.
 Require Import sflib.
 (* newly added *)
-Require Export Asmgenproof.
-Require Import ModSem SimModSem SimSymbId SimMemId SimSymbId.
+Require Export Asmgenproof AsmgenproofC0 AsmgenproofC1.
+Require Import ModSem SimModSem SimSymbId SimMemExtends SimSymbId MemoryC.
+
+Require Import Skeleton Mod ModSem SimMod SimSymb SimMem AsmregsC MatchSimModSem.
+
+Local Opaque Z.mul.
 
 Set Implicit Arguments.
 
-
 Section PRESERVATION.
 
+Variable skenv_link_src skenv_link_tgt: SkEnv.t.
 Variable prog: Mach.program.
 Variable tprog: Asm.program.
 Hypothesis TRANSF: match_prog prog tprog.
 
-Definition msp: ModSemPair.t :=
-  ModSemPair.mk (MachC.modsem return_address_offset prog) (AsmC.modsem tprog) tt.
+Let ge := (SkEnv.revive (SkEnv.project skenv_link_src (defs prog)) prog).
+Let tge := (SkEnv.revive (SkEnv.project skenv_link_tgt (defs tprog)) tprog).
 
-Theorem sim
+Variable sm_link: SimMem.t.
+Hypothesis (SIMSKENVLINK: exists ss_link, SimSymb.sim_skenv sm_link ss_link skenv_link_src skenv_link_tgt).
+
+Definition msp: ModSemPair.t :=
+  ModSemPair.mk (SM := SimMemExtends)
+                (MachC.modsem return_address_offset skenv_link_src prog)
+                (AsmC.modsem skenv_link_tgt tprog) tt sm_link.
+
+Definition get_rs (ms: Mach.state) : Mach.regset :=
+  match ms with
+  | Mach.State _ _ _ _ rs _ => rs
+  | Callstate _ _ rs _ => rs
+  | Returnstate _ rs _ => rs
+  end.
+
+Record agree_eq (ms: Mach.regset) (sp: val) (rs: Asm.regset) : Prop := mkagree {
+  agree_sp: rs#SP = sp;
+  agree_sp_def: sp <> Vundef;
+  agree_mregs: forall r: mreg, (ms r) = (rs#(preg_of r))
+}.
+
+Inductive match_init_data init_sp init_ra
+          init_rs_src init_sg_src init_rs_tgt : Prop :=
+| match_init_data_intro
+    (INITRA: init_ra = init_rs_tgt RA)
+    (INITRAPTR: wf_RA (init_ra))
+    (INITRS: agree_eq init_rs_src init_sp init_rs_tgt)
+    (SIG: exists skd, skenv_link_tgt.(Genv.find_funct) (init_rs_tgt PC) = Some skd /\ SkEnv.get_sig skd = init_sg_src)
+.
+
+Inductive match_states
+          (sm_init: SimMem.t)
+          (idx: nat) (st_src0: MachC.state) (st_tgt0: AsmC.state)
+          (sm0: SimMem.t): Prop :=
+| match_states_intro
+    init_sp init_ra
+    (INITDATA: match_init_data
+                 init_sp init_ra
+                 st_src0.(MachC.init_rs) st_src0.(init_sg) st_tgt0.(init_rs))
+    (MATCHST: AsmgenproofC1.match_states ge init_sp init_ra st_src0.(MachC.st) st_tgt0)
+    (MCOMPATSRC: st_src0.(MachC.st).(MachC.get_mem) = sm0.(SimMem.src))
+    (MCOMPATTGT: st_tgt0.(get_mem) = sm0.(SimMem.tgt))
+    (IDX: measure st_src0.(MachC.st) = idx)
+.
+
+Lemma asm_step_dstep init_rs st0 st1 tr
+      (STEP: Asm.step tge st0 tr st1)
+  :
+    Simulation.DStep (modsem skenv_link_tgt tprog)
+                     (mkstate init_rs st0) tr
+                     (mkstate init_rs st1).
+Proof.
+  econs.
+  - eapply modsem_determinate.
+  - econs; auto.
+Qed.
+
+Lemma asm_star_dstar init_rs st0 st1 tr
+      (STEP: star Asm.step tge st0 tr st1)
+  :
+    Simulation.DStar (modsem skenv_link_tgt tprog)
+                     (mkstate init_rs st0) tr
+                     (mkstate init_rs st1).
+Proof.
+  induction STEP; econs; eauto.
+  eapply asm_step_dstep; auto.
+Qed.
+
+Lemma asm_plus_dplus init_rs st0 st1 tr
+      (STEP: plus Asm.step tge st0 tr st1)
+  :
+    Simulation.DPlus (modsem skenv_link_tgt tprog)
+                     (mkstate init_rs st0) tr
+                     (mkstate init_rs st1).
+Proof.
+  inv STEP. econs; eauto.
+  - eapply asm_step_dstep; eauto.
+  - eapply asm_star_dstar; eauto.
+Qed.
+
+Lemma MATCH_GENV: Genv.match_genvs (match_globdef (fun _ f tf => transf_fundef f = OK tf) eq prog) ge tge.
+Proof.
+Admitted.
+
+Theorem unfree_parallel_extends:
+  forall m1 m2 b lo hi m1',
+  Mem.extends m1 m2 ->
+  Mem_unfree m1 b lo hi = Some m1' ->
+  exists m2',
+     Mem_unfree m2 b lo hi = Some m2'
+  /\ Mem.extends m1' m2'.
+Proof.
+Admitted.
+
+Lemma revive_signature v fd
+      (FIND: Genv.find_funct tge v = Some (Internal fd))
+  :
+      Genv.find_funct skenv_link_tgt v = Some (Internal fd.(fn_sig)).
+Admitted.
+
+Lemma revive_none v
+      (FIND: Genv.find_funct skenv_link_tgt v = None)
+  :
+    Genv.find_funct tge v = None.
+Admitted.
+
+Lemma sim_skd_src skd v_src v_tgt (LE: Val.lessdef v_src v_tgt)
+      (FIND: Genv.find_funct skenv_link_src v_src = Some skd)
+  :
+    Genv.find_funct skenv_link_tgt v_tgt = Some skd.
+Admitted.
+
+Lemma sim_external v
+      (FIND: Genv.find_funct ge v = None)
+  :
+    Genv.find_funct tge v = None.
+Proof.
+Admitted.
+
+Lemma sim_find_funct_ptr b fd_src fd_tgt
+      (FINDSRC: Genv.find_funct_ptr ge b = Some (Internal fd_src))
+      (FINDTGT: Genv.find_funct_ptr tge b = Some (Internal fd_tgt))
+  :
+      fd_tgt.(fn_sig) = fd_src.(Mach.fn_sig).
+Admitted.
+
+Lemma sim_find_funct_ptr2 b fd_src
+      (FINDSRC: Genv.find_funct_ptr ge b = Some (Internal fd_src))
+  :
+    exists fd_tgt,
+      <<FINDF: Genv.find_funct_ptr tge b = Some (Internal fd_tgt)>> /\
+      <<SIGEQ: fd_tgt.(fn_sig) = fd_src.(Mach.fn_sig)>>.
+Admitted.
+
+Lemma sim_find_funct v_src v_tgt fd_src fd_tgt (LE: Val.lessdef v_src v_tgt)
+      (FINDSRC: Genv.find_funct ge v_src = Some (Internal fd_src))
+      (FINDTGT: Genv.find_funct tge v_tgt = Some (Internal fd_tgt))
+  :
+      fd_tgt.(fn_sig) = fd_src.(Mach.fn_sig).
+Proof.
+  destruct v_src, v_tgt; ss. inv LE. des_ifs.
+  eapply sim_find_funct_ptr; eauto.
+Qed.
+Lemma sim_find_funct2 v_src v_tgt fd_src (LE: Val.lessdef v_src v_tgt)
+      (FINDSRC: Genv.find_funct ge v_src = Some (Internal fd_src))
+  :
+    exists fd_tgt,
+      <<FINDF: Genv.find_funct tge v_tgt = Some (Internal fd_tgt)>> /\
+      <<SIGEQ: fd_tgt.(fn_sig) = fd_src.(Mach.fn_sig)>>.
+Proof.
+  destruct (v_src); ss. des_ifs. inv LE.
+  exploit sim_find_funct_ptr2; eauto.
+Qed.
+
+Theorem sim_modsem
   :
     ModSemPair.sim msp
 .
 Proof.
-  admit "try this!".
-Qed.
+  eapply match_states_sim with (match_states := match_states)
+                               (match_states_at := top4); eauto; ii.
 
+  - apply lt_wf.
+
+  - destruct sm_arg, args_src, args_tgt. inv SIMARGS. ss. clarify.
+    inv INITTGT. des. ss. clarify. inv RAPTR.
+    assert (SRCSTORE: exists rs_src m_src,
+               MachC.store_arguments src rs_src vs (fn_sig fd) m_src /\
+           agree_eq rs_src (Vptr (Mem.nextblock src)
+                          Ptrofs.zero true) rs /\ Mem.extends m_src m).
+    { admit "". } destruct SRCSTORE as [rs_src [m_src [SRCSTORE [AGREE EXTENDS]]]].
+    inv AGREE.
+    exists (MachC.mkstate
+              rs_src (fn_sig fd)
+              (Callstate
+                 [dummy_stack
+                    (Vptr (Mem.nextblock src)
+                          Ptrofs.zero true) (rs RA)]
+                 fptr rs_src m_src)). esplits; auto.
+    inv SAFESRC. ss.
+    + econs; auto.
+      * eapply sim_find_funct; eauto.
+      * ss.
+      * ii. exploit PTRFREE; eauto.
+        eapply Asm.to_preg_to_mreg.
+        rewrite (agree_mregs0 mr) in *. auto.
+    + instantiate (1:= mk m_src m).
+      econs; ss; econs; ss; eauto; try by (econs; eauto).
+      * exists (Internal fd.(fn_sig)). esplits; auto.
+        eapply revive_signature. auto.
+      * econs; ss.
+        i. rewrite agree_mregs0. econs.
+
+  - ss. des. inv SIMARGS. destruct sm_arg. ss. clarify.
+    inv SAFESRC.
+    exploit sim_find_funct2; eauto. i. des.
+    assert (exists rs_tgt m_tgt,
+               <<STORE: AsmC.store_arguments (Args.m args_tgt) rs_tgt (Args.vs args_tgt)
+                                    (fn_sig fd_tgt) m_tgt>> /\
+               <<RSPC: rs_tgt PC = Args.fptr args_tgt>> /\
+               <<RSRA: rs_tgt RA = Vnullptr>> /\
+               <<PTRFREE: forall (pr : preg) (mr : mreg),
+                 Asm.to_mreg pr = Some mr ->
+                 ~ In (R mr) (regs_of_rpairs (loc_arguments (fn_sig fd_tgt))) ->
+                 ~ ValuesC.is_real_ptr (rs_tgt pr)>>).
+    { admit "". } des.
+    eexists. econs; eauto.
+    + rewrite SIGEQ. auto.
+    + rewrite RSRA. econs; ss.
+
+  - inv MATCH; ss. destruct st_src0, st_tgt0, sm0. ss. inv MATCHST; ss.
+
+  - ss. inv CALLSRC. inv MATCH. inv INITDATA. inv MATCHST. ss.
+    destruct st_tgt0. ss. clarify.
+    des.
+    inv FPTR; ss. destruct (rs0 PC) eqn:PCEQ; ss. des_ifs.
+    exploit Asmgenproof0.extcall_arguments_match; eauto. intros TGRARGS. des.
+    exploit Mem.free_parallel_extends; eauto. intros TGTFREE. des.
+    esplits; ss.
+    + econs; eauto.
+      * eapply sim_external. ss.
+      * exists skd0. des_ifs. esplits; auto.
+        eapply sim_skd_src. econs. ss.
+      * inv AG. rewrite agree_sp0. clarify.
+      * inv INITRAPTR. inv STACKS; ss.
+        -- inv ATLR; auto. exfalso; auto.
+        -- destruct ra; ss; try inv H0. inv ATLR. ss.
+    + instantiate (1:=mk m1 m2'). econs; ss; eauto.
+    + ss.
+
+  - inv AFTERSRC. ss. des. clarify. destruct st_tgt0, st. inv MATCH. inv MATCHST.
+    inv INITDATA. inv SIMRET. destruct sm_ret. ss. clarify.
+    exploit unfree_parallel_extends; try eapply UNFREE; eauto.
+    intros TRTUNFREE. des.
+    esplits; auto.
+    + econs.
+      * exists skd. esplits; eauto.
+        replace (r PC) with fptr; auto.
+        { eapply sim_skd_src. econs. eauto. }
+        inv FPTR; ss.
+      * ss.
+      * inv AG. rewrite agree_sp0. eauto.
+      * eauto.
+    + instantiate (1:= mk m1 m2'). inv INITRS. inv AG.
+      econs; ss; eauto; econs; eauto.
+      econs; eauto.
+      unfold loc_external_result, regset_after_external, Mach.regset_after_external.
+      apply agree_set_other; auto. apply agree_set_pair; auto.
+      econstructor; ss; eauto.
+      intros. rewrite to_preg_to_mreg.
+      destruct (Conventions1.is_callee_save r0) eqn:T; eauto.
+  - ss. inv FINALSRC. des. clarify. destruct st_tgt0, st. inv MATCH. inv MATCHST.
+    inv INITDATA. destruct sm0. ss. clarify.
+    exploit Mem.free_parallel_extends; eauto. intros TGTFREE. des.
+    esplits; auto.
+    + econs.
+      * inv INITRS. inv AG.
+        i. eapply Val.lessdef_trans. rewrite <- agree_mregs0.
+        eapply CALLEESAVE; auto. auto.
+      * inv INITRS. inv STACKS; [|inv H7]; rewrite H0. ss.
+      * exists skd. instantiate (1:=init_sg). esplits; auto.
+      * instantiate (1 := m2'). eauto.
+      * eapply RETV.
+      * inv STACKS; [|inv H7].
+        replace (r PC) with (init_rs0 RA).
+        { inv INITRAPTR. destruct (init_rs0 RA); ss. des_ifs. }
+        inv ATPC; auto.
+        inv INITRAPTR. exfalso. auto.
+      * inv STACKS; [|inv H7].
+        inv ATPC; auto. inv INITRAPTR. exfalso. auto.
+      * eauto.
+      * inv INITRS. inv AG.
+        rewrite agree_sp0.
+        inv STACKS; [|inv H7]; rewrite H0. ss.
+    + econs; simpl.
+      * ss. inv AG. auto.
+      * instantiate (1:= mk _ _). ss.
+      * ss.
+    + ss.
+
+  - ss. esplits.
+    + eapply MachC.modsem_receptive.
+      intros f c ofs of' RAO0 RAO1. inv RAO0. inv RAO1.
+      rewrite TC in *. rewrite TF in *. clarify.
+      exploit code_tail_unique. apply TL. apply TL0.
+      intros EQ. destruct ofs, of'. ss. clarify.
+      f_equal. apply proof_irrelevance.
+
+    + i. inv STEPSRC. inv MATCH. set (INITDATA0 := INITDATA). inv INITDATA0.
+      inv INITRAPTR. inv INITRS0. clarify.
+      exploit step_simulation; ss; try apply agree_sp_def0; eauto.
+      { apply MATCH_GENV. }
+      i. des; ss; esplits; auto; clarify.
+      * left. instantiate (1 := mkstate st_tgt0.(init_rs) S2'). ss.
+        destruct st_tgt0. eapply asm_plus_dplus; eauto.
+      * instantiate (1 := mk (MachC.get_mem (MachC.st st_src1)) (get_mem S2')).
+        econs; ss; eauto.
+        rewrite <- INITRS. rewrite <- INITFPTR. auto.
+      * right. split; eauto. apply star_refl.
+      * instantiate (1 := mk (MachC.get_mem (MachC.st st_src1))
+                             st_tgt0.(st).(get_mem)).
+        econs; ss; eauto.
+        rewrite <- INITRS. rewrite <- INITFPTR. auto.
+
+  Unshelve. apply 0%nat.
+Qed.
+    
 End PRESERVATION.
