x86/AsmgenproofC0.v
@@ -1,0 +1,70 @@
+(* *********************************************************************)
+(*                                                                     *)
+(*              The Compcert verified compiler                         *)
+(*                                                                     *)
+(*          Xavier Leroy, INRIA Paris-Rocquencourt                     *)
+(*                                                                     *)
+(*  Copyright Institut National de Recherche en Informatique et en     *)
+(*  Automatique.  All rights reserved.  This file is distributed       *)
+(*  under the terms of the INRIA Non-Commercial License Agreement.     *)
+(*                                                                     *)
+(* *********************************************************************)
+
+(** Correctness proof for Asm generation: machine-independent framework *)
+
+Require Import Coqlib.
+Require Intv.
+Require Import AST.
+Require Import Errors.
+Require Import Integers.
+Require Import Floats.
+Require Import Values.
+Require Import Memory.
+Require Import Globalenvs.
+Require Import Events.
+Require Import Smallstep.
+Require Import Locations.
+Require Import MachC Mach.
+Require Import Asm.
+Require Import Asmgen.
+Require Import Conventions.
+Require Import sflib Asmgenproof0.
+
+(** * Processor registers and register states *)
+
+Section MATCH_STACK.
+
+Variable ge: Mach.genv.
+Variable initial_parent_sp : val.
+Hypothesis initial_parent_sp_def : initial_parent_sp <> Vundef.
+Variable initial_parent_ra : val.
+Hypothesis initial_parent_ra_ptr : Val.has_type initial_parent_ra Tptr.
+Hypothesis initial_parent_ra_fake : ~ ValuesC.is_real_ptr initial_parent_ra.
+
+Inductive match_stack: list Mach.stackframe -> Prop :=
+  | match_stack_dummy
+    :
+      match_stack ((dummy_stack initial_parent_sp initial_parent_ra)::[])
+  | match_stack_cons: forall fb sp ra c s f tf tc,
+      Genv.find_funct_ptr ge fb = Some (Internal f) ->
+      transl_code_at_pc ge ra fb f c false tf tc ->
+      sp <> Vundef ->
+      match_stack s ->
+      match_stack (Stackframe fb sp ra c :: s).
+
+Lemma parent_sp_def: forall s, match_stack s -> parent_sp s <> Vundef.
+Proof.
+  induction 1; simpl.
+  unfold Vnullptr; destruct Archi.ptr64; congruence.
+  auto.
+Qed.
+
+Lemma lessdef_parent_sp:
+  forall s v,
+  match_stack s -> Val.lessdef (parent_sp s) v -> v = parent_sp s.
+Proof.
+  intros. inv H0. auto. exploit parent_sp_def; eauto. tauto.
+Qed.
+
+End MATCH_STACK.
+
