x86/LowerBound.v
@@ -1,0 +1,1251 @@
+Require Import CoqlibC Maps.
+Require Import ASTC Integers Floats Values MemoryC Events Globalenvs Smallstep.
+Require Import Locations Stacklayout Conventions Linking.
+(** newly added **)
+Require Export Asm.
+Require Import Simulation Memory ValuesC.
+Require Import Skeleton ModSem Mod sflib AsmC Sem Syntax LinkingC Program SemProps.
+Require Import MemoryC2 Lia.
+
+Set Implicit Arguments.
+
+Local Opaque Z.mul.
+
+Section PRESERVATION.
+
+  Existing Instance Val.mi_final.
+
+(** ********************* linking *********************************)
+  
+  Variable progs : list Asm.program.
+  Let prog : Syntax.program := List.map AsmC.module progs.
+
+  Variable tprog : Asm.program.
+  Hypothesis LINK : link_list progs = Some tprog.
+  (* TODO: tprog always exists *)
+
+(** ********************* genv *********************************)
+  
+  Variable sk : Sk.t.
+  Hypothesis LINK_SK : link_sk prog = Some sk.
+  (* TODO: consider linking fail case *)
+  Let skenv_link := Sk.load_skenv sk.
+  Let ge := load_genv prog skenv_link.
+  Let tge := Genv.globalenv tprog.
+
+  Definition local_genv (p : Asm.program) :=
+    (skenv_link.(SkEnv.project) p.(defs)).(SkEnv.revive) p.
+
+  Inductive genv_le (j: meminj) (src_ge tgt_ge: Genv.t fundef unit): Prop :=
+  | genv_le_intro 
+      (SYMB: forall id b (FIND: Genv.find_symbol src_ge id = Some b),
+          Genv.find_symbol tgt_ge id = Some b
+          /\ j b = Some (b, 0)) (* is it needed? *)
+      (DEFS: forall b0 d (FIND: Genv.find_def src_ge b0 = Some d),
+          exists b1, j b0 = Some (b1, 0)
+                     /\ Genv.find_def tgt_ge b1 = Some d).
+
+  Lemma genv_le_incr j0 j1 src_ge tgt_ge
+        (INCR: inject_incr j0 j1)
+        (GENVLE: genv_le j0 src_ge tgt_ge)
+    :      
+       genv_le j1 src_ge tgt_ge.
+  Proof.
+    inv GENVLE. econs; ii; ss.
+    - specialize (SYMB _ _ FIND). des. eauto.
+    - specialize (DEFS _ _ FIND). des. esplits; eauto.
+  Qed.
+
+  Lemma symb_preserved id
+    :
+      Senv.public_symbol (symbolenv (semantics tprog)) id =
+      Senv.public_symbol (symbolenv (sem prog)) id.
+  Proof.
+  Admitted.
+
+  Lemma symb_main :
+    Genv.find_symbol skenv_link (prog_main sk) =
+    Genv.find_symbol tge (prog_main tprog).
+  Proof.
+    unfold Genv.find_symbol in *.
+ admit "". Qed.
+
+  Lemma skenv_link_main
+    :
+      Genv.find_funct
+        skenv_link (Genv.symbol_address tge (prog_main tprog) Ptrofs.zero)
+      = Some (Internal signature_main).
+  Admitted.
+
+  Lemma local_genv_skenv_signature p fptr fd
+        (FIND: Genv.find_funct (local_genv p) fptr = Some (Internal fd))
+    :
+      Genv.find_funct skenv_link fptr = Some (Internal (fn_sig fd)).
+  Admitted.
+  
+(** ********************* initial memory *********************************)
+  
+  Variable m_init : mem.
+  Hypothesis INIT_MEM: sk.(Sk.load_mem) = Some m_init.
+  (* TODO: m_init exist *)
+
+  Definition m_tgt_init := m_init.
+  (* Variable m_tgt_init : mem. *)
+  (* Hypothesis INIT_TGT_MEM: Genv.init_mem tprog = Some m_tgt_init. *)
+  Lemma TGT_INIT_MEM: Genv.init_mem tprog = Some m_tgt_init.
+  Proof.
+    unfold Sk.load_mem in *.
+    eapply Genv.init_mem_match
+      with (ctx := tt) (match_fundef := top3) (match_varinfo := top2);
+      [| eapply INIT_MEM]. econs.
+    - admit "list_forall2 (match_ident_globdef top3 top2 ()) (prog_defs sk) (prog_defs tprog)".
+    - admit "prog_main tprog = prog_main sk /\ prog_public tprog = prog_public sk".
+  Qed.
+
+  Definition init_inject := Mem.flat_inj (Mem.nextblock m_init).
+
+  Lemma initmem_inject: Mem.inject init_inject m_init m_tgt_init.
+  Proof.
+    eapply Genv.initmem_inject. unfold Sk.load_mem in INIT_MEM. eauto.
+  Qed.
+
+  Lemma init_inject_genv_le p: genv_le init_inject (local_genv p) tge.
+  Admitted.
+
+  Lemma local_genv_le j p
+        (INCR: inject_incr init_inject j)
+    : genv_le j (local_genv p) tge.
+  Proof.
+    eapply genv_le_incr; eauto. apply init_inject_genv_le.
+  Qed.  
+
+  Definition agree (j: meminj) (rs_src rs_tgt: regset) : Prop :=
+    forall pr, Val.inject j (rs_src pr) (rs_tgt pr).
+
+  Lemma system_symbols_inject j
+        (INCR: inject_incr init_inject j)
+    :
+      symbols_inject j (System.globalenv skenv_link) tge.
+  Admitted.
+
+  Lemma external_function_sig v skd ef
+        (FIND0: Genv.find_funct (System.globalenv skenv_link) v =
+               Some (External ef))
+        (FIND1: Genv.find_funct skenv_link v = Some skd)
+    :
+      SkEnv.get_sig skd = ef_sig ef.
+  Admitted.
+
+  Lemma system_function_ofs j b_src b_tgt delta fd
+        (INCR: inject_incr init_inject j)
+        (FIND: Genv.find_funct_ptr (System.globalenv skenv_link) b_src = Some fd)
+        (INJ: j b_src = Some (b_tgt, delta))
+    :
+      delta = 0.
+  Admitted.
+
+  Lemma system_sig j b_src b_tgt delta ef
+        (INCR: inject_incr init_inject j)
+        (FIND: Genv.find_funct_ptr (System.globalenv skenv_link) b_src =
+               Some (External ef))
+        (INJ: j b_src = Some (b_tgt, delta))
+    :
+      Genv.find_funct_ptr tge b_tgt = Some (External ef).
+  Admitted.
+
+  Lemma system_receptive_at st frs
+    :
+      receptive_at (sem prog)
+                   (State ((Frame.mk (System.modsem skenv_link) st) :: frs)).
+  Admitted.
+
+  Lemma asm_determinate_at p st
+    :
+      determinate_at (semantics p) st.
+  Admitted.
+
+  Lemma system_genv_skenv v ef
+        (GEFIND: Genv.find_funct (System.globalenv skenv_link) v =
+                 Some (External ef))
+    :
+      Genv.find_funct (System.skenv skenv_link) v =
+      Some (External ef).
+  Admitted.
+
+  Lemma asm_step_preserve_injection
+        rs_src0 rs_src1 m_src0 m_src1 tr j0
+        rs_tgt0 m_tgt0
+        ge_src ge_tgt
+        (GENVLE: genv_le j0 ge_src ge_tgt)
+        (GE: genv_le j0 ge_src ge_tgt)
+        (AGREE: agree j0 rs_src0 rs_tgt0)
+        (INJ: Mem.inject j0 m_src0 m_tgt0)
+        (STEP: Asm.step ge_src (Asm.State rs_src0 m_src0) tr (Asm.State rs_src1 m_src1))
+    :
+      exists rs_tgt1 m_tgt1 j1,
+        (Asm.step ge_tgt (Asm.State rs_tgt0 m_tgt0) tr (Asm.State rs_tgt1 m_tgt1)) /\
+        (agree j1 rs_src1 rs_tgt1) /\
+        (Mem.inject j1 m_src1 m_tgt1) /\
+        (inject_incr j0 j1).
+  Admitted.
+
+  Lemma ALLOC_NEXT_INCR F V (gen: Genv.t F V) x m0 m1
+        (ALLOC: Genv.alloc_global gen m0 x = Some m1)
+    :
+      Plt (Mem.nextblock m0) (Mem.nextblock m1).
+  Proof.
+    destruct x. ss. destruct g; des_ifs.
+    - apply Mem.nextblock_alloc in Heq.
+      eapply Mem.nextblock_drop in ALLOC.
+      rewrite ALLOC. rewrite Heq. apply Plt_succ.
+    - apply Mem.nextblock_alloc in Heq.
+      apply Genv.store_zeros_nextblock in Heq0.
+      apply Genv.store_init_data_list_nextblock in Heq1.
+      eapply Mem.nextblock_drop in ALLOC.
+      rewrite ALLOC. rewrite Heq1. rewrite Heq0. rewrite Heq.
+      apply Plt_succ.
+  Qed.
+
+  Lemma ALLOCS_NEXT_INCR F V (gen: Genv.t F V) l m0 m1
+        (ALLOC: Genv.alloc_globals gen m0 l = Some m1)
+    :
+      Ple (Mem.nextblock m0) (Mem.nextblock m1).
+  Proof.
+    revert l gen m0 m1 ALLOC. induction l; i; ss; clarify.
+    - reflexivity.
+    - des_ifs. etrans.
+      + apply Plt_Ple. eapply ALLOC_NEXT_INCR; eauto.
+      + eapply IHl; eauto.
+  Qed.
+
+  Lemma init_mem_nextblock F V (p: AST.program F V) m
+        (INIT: Genv.init_mem p = Some m)
+    :
+      Plt 1 (Mem.nextblock m).
+  Proof.
+    unfold Genv.init_mem in *.
+    eapply ALLOCS_NEXT_INCR in INIT.
+    ss. apply Pos.le_succ_l. ss.
+  Qed.
+  
+(** ********************* regset *********************************)
+
+  Definition initial_regset : regset := 
+    (Pregmap.init Vundef)
+      # PC <- (Genv.symbol_address tge tprog.(prog_main) Ptrofs.zero)
+      # RA <- Vnullptr
+      # RSP <- (Vptr 1%positive Ptrofs.zero true).
+
+  Definition initial_tgt_regset := initial_regset.
+
+  Lemma update_agree j rs_src rs_tgt pr v
+        (AGREE: agree j rs_src rs_tgt)
+        (UPDATE: Val.inject j v (rs_tgt # pr))
+    :
+      agree j (rs_src # pr <- v) rs_tgt.
+  Proof.
+    destruct pr; intros pr0; specialize (AGREE pr0); destruct pr0; eauto.
+    - destruct i, i0; eauto.
+    - destruct f, f0; eauto.
+    - destruct c, c0; eauto.
+  Qed.
+
+  Lemma update_agree2 j rs_src rs_tgt pr v_src v_tgt
+        (AGREE: agree j rs_src rs_tgt)
+        (UPDATE: Val.inject j v_src v_tgt)
+    :
+      agree j (rs_src # pr <- v_src) (rs_tgt # pr <- v_tgt).
+  Proof.
+    destruct pr; intros pr0; specialize (AGREE pr0); destruct pr0; eauto.
+    - destruct i, i0; eauto.
+    - destruct f, f0; eauto.
+    - destruct c, c0; eauto.
+  Qed.
+
+  Lemma initial_regset_agree: agree init_inject initial_regset initial_tgt_regset.
+  Proof.
+    unfold initial_tgt_regset, initial_regset.
+    repeat eapply update_agree2; ss; eauto.
+    - unfold Genv.symbol_address; des_ifs. econs; eauto.
+      unfold init_inject, Mem.flat_inj. des_ifs.
+      exfalso. eapply Genv.genv_symb_range in Heq. 
+      unfold tge in *. erewrite Genv.init_mem_genv_next in Heq. eauto.
+      apply TGT_INIT_MEM. symmetry. apply Ptrofs.add_zero.
+    - econs.
+    - econs.
+      + unfold init_inject, Mem.flat_inj; des_ifs.
+        exfalso. apply n. eapply init_mem_nextblock.
+        unfold Sk.load_mem in INIT_MEM. apply INIT_MEM.
+      + symmetry. apply Ptrofs.add_zero.
+  Qed.      
+
+(** ********************* calee initial *********************************)
+
+  Definition extcall_args_reg (mr: mreg) (sg: signature):
+    {In (R mr) (regs_of_rpairs (loc_arguments sg))} +
+    {~ In (R mr) (regs_of_rpairs (loc_arguments sg))}.
+  Proof.
+    generalize (regs_of_rpairs (loc_arguments sg)). induction l.
+    - ss. tauto.
+    - ss. inv IHl; [tauto|].
+      destruct a.
+      + destruct (mreg_eq r mr); [clarify; eauto|].
+        right. intros []; clarify.
+      + right. intros []; clarify.
+  Qed.
+
+  Lemma extcall_args_callee_save_disjoint sg mr
+        (EXT: In (R mr) (regs_of_rpairs (loc_arguments sg)))
+    :
+      ~ Conventions1.is_callee_save mr.
+  Proof.
+    destruct sg. ss.
+    unfold loc_arguments in *.
+    ss. replace Archi.ptr64 with true in *; eauto.
+    assert (forall l mr p q r,
+                In (R mr) (regs_of_rpairs (loc_arguments_64 l p q r)) ->
+                ~ is_callee_save mr); eauto.
+    induction l; ss; i; destruct a; des_ifs; ss; des; eauto; inv H; ss.
+  Qed.
+
+  Definition src_init_rs sg (rs_src: regset) (rsp: val) : regset :=
+    fun (pr : PregEq.t) =>
+      match Asm.to_mreg pr with
+      | Some mr =>
+        if (extcall_args_reg mr sg)
+        then (rs_src pr)
+        else (to_fake (rs_src pr))
+      | None =>
+        match pr with
+        | IR RSP => rsp
+        | PC => rs_src PC
+        | RA => to_fake (rs_src RA)
+        | _ => to_fake (rs_src pr)
+        end
+      end.
+
+  Lemma src_init_rs_agree' j sg rsp (rs_src rs_tgt: regset)
+        (AGREE: agree j rs_src rs_tgt)
+        (RSPINJ: Val.inject j rsp (rs_tgt # RSP))
+    :
+      agree j (src_init_rs sg rs_src rsp) rs_tgt.
+  Proof.
+    intros pr. specialize (AGREE pr). unfold src_init_rs.
+    destruct pr; ss; try (destruct (extcall_args_reg _ sg); ss; eapply to_fake_inj; eauto).
+    - destruct i; try (destruct (extcall_args_reg _ sg); ss; eapply to_fake_inj; eauto); ss.
+    - destruct f; try (destruct (extcall_args_reg _ sg); ss; eapply to_fake_inj; eauto); ss.
+    - eapply to_fake_inj; eauto.
+    - eapply to_fake_inj; eauto.
+  Qed.
+
+  Lemma src_init_rs_agree j sg blk ofs new_blk (rs_src rs_tgt: regset)
+        (RSPPTR: rs_src # RSP = Vptr blk ofs true)
+        (INJNONE: j new_blk = None)
+        (AGREE: agree j rs_src rs_tgt)
+    :
+      agree (callee_injection j blk new_blk)
+            (src_init_rs sg rs_src (Vptr new_blk ofs true)) rs_tgt.
+  Proof.
+    set (RSPAGREE := AGREE RSP).
+    rewrite RSPPTR in *. inv RSPAGREE. eapply src_init_rs_agree'.
+    - intros pr. specialize (AGREE pr).
+      inv AGREE; econs; clarify; eauto; unfold callee_injection; des_ifs.
+    - unfold callee_injection. rewrite <- H1. econs; auto. des_ifs; eauto.
+  Qed.
+
+  Inductive wf_init_rs (j: meminj) (rs_caller rs_callee: regset) : Prop :=
+  | wf_init_rs_intro
+      (PCSAME: rs_caller # PC = rs_callee # PC)
+      (RAPTR: wf_RA (rs_callee # RA))
+      (RASAME: to_fake (rs_caller # RA) = rs_callee # RA)
+      (RSPSAME: inj_same j (rs_caller # RSP) (rs_callee # RSP))
+      (CALLEESAVE: forall mr, Conventions1.is_callee_save mr ->
+                              almost_eq (rs_caller (to_preg mr))
+                                        (rs_callee (to_preg mr)))
+  .    
+
+  Lemma src_init_rs_wf j old_blk new_blk ofs (rs: regset) sg b' delta
+        (INJ_NONE: j new_blk = None)
+        (INJ_SOME: j old_blk = Some (b', delta))
+        (TPTR: Val.has_type (rs RA) Tptr)
+        (RADEF: rs RA <> Vundef)
+        (RSRSP: rs # RSP = Vptr old_blk ofs true)
+        (OFSZERO: ofs = Ptrofs.zero)
+    :
+      wf_init_rs
+      (callee_injection j old_blk new_blk)
+      rs
+      (src_init_rs sg rs (Vptr new_blk ofs true)).
+  Proof.
+    econs; ss.
+    - unfold src_init_rs. ss. destruct (rs RA); des_ifs; ss. des_ifs.
+    - econs; eauto; ss.
+      + unfold callee_injection. des_ifs. apply INJ_SOME.
+      + unfold callee_injection. des_ifs.
+    - intros. unfold src_init_rs. Opaque to_fake.
+      destruct mr; ss; clarify; des_ifs; try econs; try apply to_fake_almost_eq.
+  Qed.          
+
+  Lemma preg_case pr :
+    (exists mr, pr = to_preg mr) \/
+    (pr = PC) \/ (exists c, pr = CR c) \/ (pr = RSP) \/ (pr = RA)
+  .
+  Proof.
+    destruct (to_mreg pr) eqn:EQ.
+    - left. exists m. unfold to_mreg in *.
+      destruct pr; clarify.
+      destruct i; clarify; auto.
+      destruct f; clarify; auto.
+    - right. unfold to_mreg in *.
+      destruct pr; clarify; eauto.
+      destruct i; clarify; auto.
+      destruct f; clarify; auto.
+  Qed.
+
+  Lemma callee_save_agree j rs_caller init_rs rs_callee rs_tgt sg mr rs
+        (WF: wf_init_rs j rs_caller init_rs)
+        (AGREE: agree j rs_callee rs_tgt)
+        (INITSIG: exists skd, skenv_link.(Genv.find_funct) (init_rs # PC) = Some skd /\ SkEnv.get_sig skd = sg)
+        (RETV: loc_result sg = One mr)
+        (CALLEESAVE: forall mr, Conventions1.is_callee_save mr ->
+                                Val.lessdef (init_rs mr.(to_preg)) (rs_callee mr.(to_preg)))
+        (RSRA: rs_callee # PC = init_rs # RA)
+        (RSRSP: rs_callee # RSP = init_rs # RSP)
+        (RS: rs = (set_pair (loc_external_result sg) (rs_callee mr.(to_preg)) (Asm.regset_after_external rs_caller)) #PC <- (rs_caller RA))
+    :
+        agree j rs rs_tgt.
+  Proof.
+    inv WF. clarify.
+    - unfold loc_external_result. rewrite RETV. ss.
+      eapply update_agree; eauto; cycle 1.
+      { eapply to_fake_inj2. rewrite RASAME. rewrite <- RSRA. auto. }
+      eapply update_agree; eauto.
+      unfold Asm.regset_after_external in *. intros pr. specialize (AGREE pr).
+      destruct (preg_case pr); des; clarify; ss.
+      + rewrite to_preg_to_mreg. des_ifs.
+        specialize (CALLEESAVE mr0). specialize (CALLEESAVE0 mr0).
+        rewrite Heq in *.
+        eapply almost_eq_commute with (v_src1 := init_rs (to_preg mr0)); eauto.
+        eapply lessdef_commute with (v_src1 := rs_callee (to_preg mr0)); eauto.
+      + rewrite RSRSP in *.
+        eapply inj_same_inj2; eauto.
+  Qed.
+
+(** ********************* match stack *********************************)
+  
+  Inductive match_stack (j: meminj) : regset -> list Frame.t -> Prop :=
+  | match_stack_init
+      init_rs
+      (RSRA: init_rs # RA = Vnullptr)
+      (RSPC: init_rs # PC = Genv.symbol_address tge tprog.(prog_main) Ptrofs.zero)
+      (SIG: skenv_link.(Genv.find_funct) (Genv.symbol_address tge tprog.(prog_main) Ptrofs.zero) = Some (Internal signature_main))
+    :
+      match_stack j init_rs nil
+  | match_stack_cons
+      fr frs p st init_rs0 init_rs1
+      (FRAME: fr = Frame.mk (AsmC.modsem skenv_link p) (AsmC.mkstate init_rs1 st))
+      (STACK: match_stack j init_rs1 frs)
+      (WF: wf_init_rs j st.(st_rs) init_rs0)
+    :
+      match_stack j init_rs0 (fr::frs)
+  .
+
+  Inductive match_stack_call (j: meminj) : mem -> regset -> list Frame.t -> Prop :=
+  | match_stack_call_init
+      init_rs m
+      (MEM: m = m_init)
+      (INITRS: init_rs = initial_regset)
+    :
+      match_stack_call j m init_rs nil
+  | match_stack_call_cons
+      fr frs p st init_rs0 init_rs1 m
+      (FRAME: fr = Frame.mk (AsmC.modsem skenv_link p)
+                            (AsmC.mkstate init_rs1 st))
+      (INITRS: init_rs0 = st.(st_rs))
+      (STACK: match_stack j init_rs1 frs)
+      (MEM: m = st.(st_m))      
+    :
+      match_stack_call j m init_rs0 (fr::frs)
+  .
+
+  Lemma match_stack_incr j1 j2 init_rs l
+        (INCR: inject_incr j1 j2)
+        (MATCH: match_stack j1 init_rs l)
+    :
+      match_stack j2 init_rs l.
+  Proof.
+    revert init_rs INCR MATCH. induction l; ss; ii; inv MATCH; econs; ss; eauto.
+    inv WF. econs; eauto.
+    inv RSPSAME. econs; eauto.
+  Qed.
+
+  Lemma frame_inj a0 b0 a1 b1
+        (EQ: Frame.mk a0 b0 = Frame.mk a1 b1)
+    : b0 ~= b1.
+  Proof. inv EQ. eauto. Qed.
+
+  Lemma asm_frame_inj se1 se2 p1 p2 st1 st2
+        (EQ : Frame.mk (modsem se1 p1) st1 = Frame.mk (modsem se2 p2) st2)
+    :
+      st1 = st2.
+  Proof. apply frame_inj in EQ. apply JMeq_eq. eauto. Qed.
+
+(** ********************* arguments *********************************)
+
+  Lemma src_init_rs_PTRFREE sg rs v
+    :
+      forall
+          pr mr
+          (MR: to_mreg pr = Some mr)
+          (NOTIN: ~In (R mr) (regs_of_rpairs (loc_arguments sg)))
+        ,
+          <<PTRFREE: ~ is_real_ptr ((src_init_rs sg rs v) pr)>>.
+  Proof.
+    i. intros PTR. unfold src_init_rs in PTR.
+    des_ifs; eapply to_fake_fake_ptr; eauto.
+  Qed.
+
+  Lemma src_init_rs_argument (rs: regset) m0 m1 sg rsp mr v
+        (ARG: extcall_arg rs m0 (R mr) v)
+        (IN: In (R mr) (regs_of_rpairs (loc_arguments sg)))
+    :
+      extcall_arg (src_init_rs sg rs rsp) m1 (R mr) v.
+  Proof.
+    inv ARG.
+    replace (rs (preg_of mr)) with (src_init_rs sg rs rsp (preg_of mr)); [econs|].
+    unfold src_init_rs.
+    destruct mr; ss; des_ifs.
+  Qed.
+
+  Lemma arguments_loc sg sl delta ty
+        (IN: In (S sl delta ty) (regs_of_rpairs (loc_arguments sg)))
+    :
+      sl = Outgoing /\
+      0 <= delta /\
+      4 * delta + size_chunk (chunk_of_type ty) <= 4 * size_arguments sg.
+  Proof.
+    set (loc_arguments_acceptable_2 _ _ IN). ss. des_ifs.
+    set (loc_arguments_bounded _ _ _ IN).
+    splits; eauto; [omega|].
+    unfold typesize in *. des_ifs; ss; lia.
+  Qed.
+
+  Lemma tail_In A l0 l1 (a: A)
+        (IN: In a l0)
+        (TAIL: is_tail l0 l1)
+    :
+      In a l1.
+  Proof.
+    induction TAIL; auto.
+    econs 2; eauto.
+  Qed.        
+
+  Lemma memcpy_argument
+        (rs0 rs1: regset) m_src0 m_src1 m_src2 sg blk_old blk_new ofs delta ty v
+        (RSRSP0: rs0 # RSP = Vptr blk_old ofs true)
+        (RSRSP1: rs1 # RSP = Vptr blk_new ofs true)
+        (OFS: ofs = Ptrofs.zero)
+        (NEQ: blk_old <> blk_new)
+        (FREE: freed_from m_src0 m_src1 blk_old 0 (4*size_arguments sg))
+        (ALLOC: Mem.alloc m_src1 0 (4*size_arguments sg)
+                = (m_src2, blk_new))
+        (ARG: extcall_arg rs0 m_src0 (S Outgoing delta ty) v)
+        (DELTA0: 0 <= delta)
+        (SZ: 4 * size_arguments sg <= Ptrofs.modulus)
+        (DELTA1: 4 * delta + size_chunk (chunk_of_type ty) <= 4 * size_arguments sg)
+    :
+      extcall_arg
+        rs1
+        (memcpy m_src2 blk_old blk_new) (S Outgoing delta ty) v.
+  Proof.
+    clarify. econs. refl. inv ARG.
+    rewrite RSRSP0 in *. rewrite RSRSP1 in *. ss.
+    assert (CHUNK: 0 < size_chunk (chunk_of_type ty)).
+    { unfold size_chunk. destruct (chunk_of_type ty); lia. }
+    eapply memcpy_load; eauto.
+    - apply Ptrofs.unsigned_range.
+    - rewrite Ptrofs.add_zero_l. rewrite Ptrofs.unsigned_repr; [lia|].
+      unfold Ptrofs.max_unsigned. lia.
+  Qed.
+
+  Lemma init_argument (rs: regset) ofs blk_old blk_new m_src0 m_src1 m_src2 sg l v
+        (RSRSP: rs # RSP = Vptr blk_old ofs true)
+        (OFSZERO: ofs = Ptrofs.zero)
+        (NEQ: blk_old <> blk_new)
+        (FREE: freed_from m_src0 m_src1 blk_old 0 (4*size_arguments sg))
+        (ALLOC: Mem.alloc m_src1 0 (4*size_arguments sg)
+                = (m_src2, blk_new))
+        (ARG: extcall_arg rs m_src0 l v)
+        (SZ: 4 * size_arguments sg <= Ptrofs.modulus)
+        (IN: In l (regs_of_rpairs (loc_arguments sg)))
+    :
+      extcall_arg (src_init_rs sg rs (Vptr blk_new ofs true))
+                  (memcpy m_src2 blk_old blk_new) l v.
+  Proof.
+    destruct l.
+    - eapply src_init_rs_argument; eauto.
+    - apply arguments_loc in IN. des. clarify.
+      eapply memcpy_argument; eauto.
+  Qed.      
+
+  Lemma regs_of_rpair_In A (l: list (rpair A))
+    :
+      (forall r (IN: In (One r) l), In r (regs_of_rpairs l))
+      /\ (forall r0 r1 (IN: In (Twolong r0 r1) l),
+             In r0 (regs_of_rpairs l) /\ In r1 (regs_of_rpairs l)).
+  Proof.
+    induction l; i; ss; split; i; des; clarify; ss; eauto.
+    - eapply in_or_app. eauto.
+    - split; eapply in_or_app; right; eapply (IHl0 _ _ IN).
+  Qed.
+
+  Lemma memcpy_store_arguments
+        rs m_src0 m_src1 m_src2 sg args blk_old blk_new ofs
+        (ARGS: extcall_arguments rs m_src0 sg args)
+        (RSRSP: rs # RSP = Vptr blk_old ofs true)
+        (OFSZERO: ofs = Ptrofs.zero)
+        (NEQ: blk_old <> blk_new)
+        (SZ: 4 * size_arguments sg <= Ptrofs.modulus)
+        (FREE: freed_from m_src0 m_src1
+                          blk_old ofs.(Ptrofs.unsigned)
+                                        (ofs.(Ptrofs.unsigned)+4*size_arguments sg))
+        (ALLOC: Mem.alloc m_src1 ofs.(Ptrofs.unsigned)
+                                       (ofs.(Ptrofs.unsigned)+4*size_arguments sg)
+                = (m_src2, blk_new))
+    :
+      store_arguments
+        m_src1
+        (src_init_rs sg rs (Vptr blk_new ofs true))
+        args sg (memcpy m_src2 blk_old blk_new).
+  Proof.
+    clarify; econs; eauto.
+    - unfold extcall_arguments in *.
+      revert args ARGS. generalize (is_tail_refl (loc_arguments sg)).
+      assert (forall
+                 l args
+                 (TAIL: is_tail l (loc_arguments sg))
+                 (ARGS: list_forall2 (extcall_arg_pair rs m_src0) l args)
+               ,
+                 list_forall2
+                   (extcall_arg_pair (src_init_rs sg rs (Vptr blk_new Ptrofs.zero true))
+                                     (memcpy m_src2 blk_old blk_new)) l args); auto.
+      induction l; i; inv ARGS; econs; eauto.
+      + inv H1; econs.
+        * eapply init_argument; eauto.
+          apply tail_In with (a := One l0) in TAIL; [|econs; eauto].
+          eapply regs_of_rpair_In in TAIL. auto.
+        * eapply init_argument; eauto.
+          apply tail_In with (a := Twolong hi lo) in TAIL; [|econs; eauto].
+          eapply regs_of_rpair_In in TAIL. tauto.
+        * eapply init_argument; eauto.
+          apply tail_In with (a := Twolong hi lo) in TAIL; [|econs; eauto].
+          eapply regs_of_rpair_In in TAIL. tauto.
+      + eapply IHl; auto.
+        eapply is_tail_trans; eauto. econs 2. econs 1.
+    - econs; ss; eauto.
+      + refl.
+      + intros b ofs0 IN PERM. des_ifs.
+        * exfalso. apply IN. eapply Mem.perm_alloc_3; eauto.
+        * f_equal. eapply PMap.gso; auto.
+    - ss. ii. unfold Mem.perm. ss.
+      eapply Mem.perm_alloc_2; eauto.
+  Qed.    
+
+  Local Opaque Mem.alloc.
+
+(** ********************* match states *********************************)
+
+  Definition different_owner (v0 v1 : val): Prop :=
+    forall mod0 mod1
+      (OWNER0: ge.(Ge.find_fptr_owner) v0 mod0)
+      (OWNER1: ge.(Ge.find_fptr_owner) v1 mod1),
+      mod0 <> mod1.
+
+  Inductive match_states : Sem.state -> Asm.state -> nat -> Prop :=
+  | match_states_intro
+      j fr frs p init_rs rs_src rs_tgt m_src m_tgt n
+      (AGREE: agree j rs_src rs_tgt)
+      (INJ: Mem.inject j m_src m_tgt)
+      (INITINCR: inject_incr init_inject j)
+      (FRAME: fr = Frame.mk (AsmC.modsem skenv_link p)
+                            (AsmC.mkstate init_rs (Asm.State rs_src m_src)))
+      (STACK: match_stack j init_rs frs)
+      (* (RAPTR: wf_RA (init_rs RA)) *)
+      (ORD: n = if (external_state (local_genv p) (rs_src # PC))
+                then (length frs + 2)%nat else 0%nat)
+    :
+      match_states (State (fr::frs)) (Asm.State rs_tgt m_tgt) n
+  | match_states_call
+      j init_rs frs args m_src rs_tgt m_tgt ofs blk sg n
+      (STACK: match_stack_call j m_src init_rs frs)
+      (AGREE: agree j init_rs rs_tgt)
+      (INJECT: Mem.inject j m_src m_tgt)
+      (INITINCR: inject_incr init_inject j)
+      (FPTR: args.(Args.fptr) = init_rs # PC)
+      (SIG: exists skd, skenv_link.(Genv.find_funct) args.(Args.fptr)
+                        = Some skd /\ SkEnv.get_sig skd = sg)
+      (ARGS: extcall_arguments init_rs m_src sg args.(Args.vs))
+      (RSPPTR: init_rs # RSP = Vptr blk ofs true)
+      (OFSZERO: ofs = Ptrofs.zero)
+      (* (RAPTR: wf_RA (init_rs RA)) *)
+      (RAPTR: <<TPTR: Val.has_type (init_rs RA) Tptr>> /\ <<RADEF: init_rs RA <> Vundef>>)
+      (FREE: freed_from m_src args.(Args.m) blk ofs.(Ptrofs.unsigned) (ofs.(Ptrofs.unsigned) + 4 * (size_arguments sg)))
+      (ORD: n = 1%nat)
+    :
+      match_states (Callstate args frs) (Asm.State rs_tgt m_tgt) n.
+
+
+(** ********************* transf initial final  *********************************)
+
+  Lemma transf_initial_states:
+    forall st1, Sem.initial_state prog st1 ->
+                exists st2, Asm.initial_state tprog st2 /\ match_states st1 st2 1.
+  Proof.
+    generalize TGT_INIT_MEM.
+    generalize initial_regset_agree.
+    generalize initmem_inject.
+    intros initmem_inject initial_regset_agree TGT_INT_MEM.
+    intros st1 INIT. inv INIT; clarify. esplits.
+    - econs; eauto.
+    - econs; ss; eauto; ss.
+      + econs; ss; eauto.
+      + unfold initial_regset.
+        rewrite Pregmap.gso; clarify.
+        rewrite Pregmap.gso; clarify. ss.
+        rewrite Pregmap.gss. unfold tge.
+        set (MAIN:= symb_main).
+        unfold Genv.symbol_address. unfold skenv_link, tge in *. rewrite MAIN. auto.
+      + econs.
+      + apply init_mem_freed_from.
+  Qed.
+
+  Lemma transf_final_states:
+    forall st1 st2 r n,
+      match_states st1 st2 n -> Sem.final_state st1 r -> Asm.final_state st2 r.
+  Proof.
+    intros st_src st_tgt r n MTCHST FINAL. inv FINAL. inv MTCHST. ss.
+    inv FINAL0. clarify. inv STACK. econs.
+    - specialize (AGREE PC). rewrite RSRA in *. rewrite RSRA0 in *.
+      inv AGREE; ss.
+    - des. rewrite RSPC in *. rewrite SIG in *. clarify.
+      ss. unfold signature_main, loc_arguments, loc_result in *.
+      Transparent Archi.ptr64. ss. unfold loc_result_64 in *. ss. clarify.
+      ss. specialize (AGREE RAX). rewrite INT in *. inv AGREE; auto.
+  Qed.  
+
+(** ********************* transf step  *********************************)
+
+  Lemma asm_step_internal_simulation
+        st_src0 st_src1 st_tgt0 tr frs p init_rs n0
+        (STEP: Asm.step (local_genv p) st_src0 tr st_src1)
+        (MTCHST: match_states (State ((Frame.mk (AsmC.modsem skenv_link p)
+                                                (AsmC.mkstate init_rs st_src0))::frs))
+                              st_tgt0 n0)
+    :
+      exists st_tgt1 n1,
+        Asm.step tge st_tgt0 tr st_tgt1 /\
+        match_states (State ((Frame.mk (AsmC.modsem skenv_link p)
+                                       (AsmC.mkstate init_rs st_src1))::frs))
+                     st_tgt1 n1.
+  Proof. 
+    inv MTCHST. apply asm_frame_inj in FRAME. clarify. destruct st_src1.
+    exploit asm_step_preserve_injection; ss; eauto.
+    - apply local_genv_le. ss.
+    - apply local_genv_le; auto.
+    - ii. des. esplits; eauto; econs; eauto.
+      + etrans. apply INITINCR. auto.
+      + eapply match_stack_incr; eauto.
+  Qed.
+
+  Lemma step_internal_simulation
+        fr0 frs tr st0 st_tgt0 n0
+        (STEP: fr0.(Frame.ms).(ModSem.step) fr0.(Frame.ms).(ModSem.globalenv) fr0.(Frame.st) tr st0)
+        (MTCHST: match_states (State (fr0 :: frs)) st_tgt0 n0) 
+    :
+      exists st_tgt1 n1,
+        Asm.step tge st_tgt0 tr st_tgt1 /\
+        match_states (State ((fr0.(Frame.update_st) st0) :: frs)) st_tgt1 n1.
+  Proof.
+    inv MTCHST. inv STEP.
+    exploit asm_step_internal_simulation; ss; eauto.
+    - econs; eauto.
+    - ii. des. esplits; ss; eauto.
+      destruct st0; ss; clarify. eassumption.
+  Qed.
+
+  Lemma step_return_simulation
+        fr0 fr1 frs retv st0 st_tgt n0
+        (FINAL: fr0.(Frame.ms).(ModSem.final_frame) fr0.(Frame.st) retv)
+        (AFTER: fr1.(Frame.ms).(ModSem.after_external) fr1.(Frame.st) retv st0)
+        (MTCHST: match_states (State (fr0 :: fr1 :: frs)) st_tgt n0)
+    :
+      exists n1, match_states (State ((fr1.(Frame.update_st) st0) :: frs)) st_tgt n1
+                 /\ (n1 < n0)%nat.
+  Proof.
+    inv MTCHST. inv STACK. ss. inv FINAL. inv AFTER. set WF as WF2. inv WF2. ss.
+    inv RSPSAME. rewrite RSRSP0 in *. rewrite INITRSP in *. clarify.
+    rewrite PCSAME in *. des. ss. clarify. esplits.
+    econs; simpl in *.
+    - eapply callee_save_agree; eauto.
+      etrans; eauto. 
+    - eapply unfree_free_inj; eauto. 
+      + instantiate (1 := Ptrofs.zero).
+        rewrite Ptrofs.unsigned_zero. rewrite Z.add_0_l.
+        apply FREE.
+      + econs; eauto.
+    - ss.
+    - ss.
+    - ss.
+    - ss.
+    - des_ifs. omega.
+  Qed.
+
+  Lemma step_call_simulation
+        fr0 frs args st_tgt n
+        (AT: fr0.(Frame.ms).(ModSem.at_external) fr0.(Frame.st) args)
+        (MTCHST: match_states (State (fr0 :: frs)) st_tgt n)
+    :
+        match_states (Callstate args (fr0 :: frs)) st_tgt 1%nat.
+  Proof.
+    inv MTCHST. ss. inv AT.
+    econs; ss; eauto.
+    - econs; eauto.
+    - eapply free_freed_from; eauto.
+  Qed.
+
+  Inductive valid_owner fptr (p: Asm.program) : Prop :=
+  | valid_owner_intro
+      fd
+      (MSFIND: ge.(Ge.find_fptr_owner) fptr (AsmC.modsem skenv_link p))
+      (FINDF: Genv.find_funct (local_genv p) fptr = Some (Internal fd))
+      (SIZEWF: 4 * size_arguments (fn_sig fd) <= Ptrofs.modulus).   
+  
+  Lemma asm_step_init_simulation
+        args frs st_tgt p n
+        (MTCHST: match_states (Callstate args frs) st_tgt n)
+        (OWNER: valid_owner args.(Args.fptr) p)
+    :
+      exists rs m,
+        (AsmC.initial_frame skenv_link p args (AsmC.mkstate rs (Asm.State rs m))) /\
+        (match_states (State ((Frame.mk (AsmC.modsem skenv_link p) (AsmC.mkstate rs (Asm.State rs m))) :: frs)) st_tgt 0).
+  Proof.
+    inv MTCHST. inv OWNER. des. ss.
+    set (nextblock_unvalid := nextblock_unvalid INJECT).
+    destruct (Mem.alloc args.(Args.m) 0 (4 * size_arguments (fn_sig fd))) eqn:MEQ.
+    set (SKDSG:= local_genv_skenv_signature _ _ FINDF). clarify. ss.
+    exists (src_init_rs (fn_sig fd) init_rs (Vptr b Ptrofs.zero true)).
+    exists (memcpy m blk b).
+    assert (BNEQ: blk <> b).
+    { intros BEQ. rewrite (Mem.alloc_result _ _ _ _ _ MEQ) in BEQ.
+      clarify. specialize (AGREE RSP). rewrite RSPPTR in *.
+      inv AGREE. rewrite (freed_from_nextblock FREE) in *. clarify.
+    }    esplits; eauto.
+    - econs.
+      + apply (eq_refl (fn_sig fd)).
+      + apply FINDF.
+      + ss.
+      + ss.
+      + eapply memcpy_store_arguments; ss; eauto.
+      + unfold src_init_rs. ss.
+        destruct (init_rs RA); ss; eauto. destruct b1; ss; eauto.
+      + apply src_init_rs_PTRFREE.
+    - rewrite <- (freed_from_nextblock FREE) in *.
+      rewrite <- (Mem.alloc_result _ _ _ _ _ MEQ) in *.
+      econs.
+      + instantiate (2 := callee_injection j blk b).
+        eapply src_init_rs_agree; eauto.
+      + eapply memcpy_inject; eauto.
+      + eapply inject_incr_trans with (f2 := j); auto.
+        apply callee_injection_incr; auto.
+      + reflexivity.
+      + inv STACK; econs; ss; [apply skenv_link_main| |].
+        * eapply match_stack_incr; [|eauto].
+          apply callee_injection_incr; auto.
+        * set (AGREERSP := AGREE RSP).
+          rewrite RSPPTR in AGREERSP. inv AGREERSP.
+          eapply src_init_rs_wf; eauto.
+      + unfold external_state.
+        des_ifs; exfalso; unfold src_init_rs, local_genv in *; ss;
+        rewrite <- FPTR in *; rewrite Heq0 in *; ss; des_ifs.
+  Qed.
+
+  Lemma step_init_simulation
+        args frs st_tgt p n
+        (MTCHST: match_states (Callstate args frs) st_tgt n)
+        (OWNER: valid_owner args.(Args.fptr) p)
+    :
+      exists st_src,
+        step ge (Callstate args frs) E0 st_src /\ match_states st_src st_tgt 0.
+  Proof.
+    exploit asm_step_init_simulation; eauto. inv OWNER.
+    i. des. esplits; try eassumption.
+    econs; eauto.
+  Qed.
+
+  Lemma at_external_external p st frs st_tgt n args
+        (MTCHST: match_states
+                   (State
+                      ((Frame.mk (AsmC.modsem skenv_link p) st)::frs))
+                   st_tgt n)
+        (ATEXTERNAL: at_external skenv_link p st args)
+    :
+      (1 < n)%nat.
+  Proof.
+    inv MTCHST.
+    replace (at_external skenv_link p) with (at_external skenv_link p0) in *.
+    - inv ATEXTERNAL. apply asm_frame_inj in FRAME. clarify.
+      unfold external_state. des_ifs. omega.
+      unfold local_genv, fundef in *. clarify.
+    - apply f_equal with (f := Frame.ms) in FRAME. ss.
+      inv FRAME. apply Eqdep.EqdepTheory.inj_pair2 in H0. auto.
+  Qed.  
+
+  Lemma normal_state_fsim_step frs st_src1 st_tgt0 t n0
+        (MTCHST: match_states (State frs) st_tgt0 n0)
+        (STEP: step ge (State frs) t st_src1)
+    :
+      (exists st_tgt1 n1,
+          Asm.step tge st_tgt0 t st_tgt1 /\ match_states st_src1 st_tgt1 n1) \/
+      (exists n1,
+          match_states st_src1 st_tgt0 n1 /\ n1 < n0)%nat /\ (t = E0).
+  Proof.
+    inv STEP.
+    - right. exploit step_call_simulation; eauto.
+      i. esplits; eauto.
+      inv MTCHST; ss.
+      exploit at_external_external; eauto.
+      econs; try eassumption; ss.
+    - left. exploit step_internal_simulation; eauto.
+    - right. exploit step_return_simulation; eauto.
+  Qed.
+
+  Lemma owner_asm_or_system fptr ms
+        (OWNER: Ge.find_fptr_owner ge fptr ms)
+    :
+      (<<ASMMOD: exists p, ms= AsmC.modsem skenv_link p >>)\/
+      (<<SYSMOD: ms = System.modsem skenv_link>>).
+  Proof.
+    inv OWNER. clear - MODSEM. unfold ge in *.
+    unfold load_genv, load_modsems, prog, flip in *.
+    ss. des; auto.
+    left. generalize progs ms MODSEM.
+    intros l. induction l; ss; i. des; eauto. 
+  Qed.
+
+  Lemma find_fptr_owner_determ
+        fptr ms0 ms1
+        (FIND0: Ge.find_fptr_owner ge fptr ms0)
+        (FIND1: Ge.find_fptr_owner ge fptr ms1)
+    :
+      ms0 = ms1
+  .
+  Proof.
+    eapply SemProps.find_fptr_owner_determ; ss;
+      rewrite LINK_SK; eauto.
+  Qed.
+
+  Lemma init_case st args frs fptr
+        (STATE: st = Callstate args frs)
+        (FPTR: fptr = args.(Args.fptr))
+    :
+      (<<ASMMOD: exists p, valid_owner fptr p>>) \/
+      (<<SYSMOD: ge.(Ge.find_fptr_owner)
+                      fptr (System.modsem skenv_link)>>) \/
+      (<<UNSAFE: ~ safe (sem prog) st>>).
+  Proof.
+    destruct (classic (exists ms, Ge.find_fptr_owner ge args.(Args.fptr) ms)) as [[ms OWNER] | NOOWNER].   
+    - destruct (owner_asm_or_system OWNER); des; clarify.
+      + destruct (classic (valid_owner args.(Args.fptr) p)); eauto.
+        right. right. intros SAFE. exploit SAFE; [econs|].
+        i. des.
+        * inv H0.
+        * inv H0. apply H.
+          revert MSFIND st_init INIT. intros MSFIND.
+          ss. rewrite LINK_SK in *.
+          rewrite <- (find_fptr_owner_determ OWNER MSFIND) in *. i.
+          inv INIT. econs; eauto.
+      + right. left. clarify.
+    - right. right. intros SAFE. clarify. exploit SAFE; [econs|].
+      i. des.
+      + inv H.
+      + inv H. ss. rewrite LINK_SK in *. eauto.
+  Qed.
+
+  Lemma call_step_noevent ge' args frs st1 tr
+        (STEP: step ge' (Callstate args frs) tr st1)
+    :
+      E0 = tr.
+  Proof. inv STEP. auto. Qed.
+
+  Lemma extcall_arg_inject j rs_src rs_tgt m_src m_tgt l v_src  
+        (AGREE: agree j rs_src rs_tgt)
+        (INJECT: Mem.inject j m_src m_tgt)
+        (ARG: extcall_arg rs_src m_src l v_src)
+    :
+      exists v_tgt,
+        extcall_arg rs_tgt m_tgt l v_tgt /\
+        Val.inject j v_src v_tgt.
+  Proof.
+    inv ARG.
+    - exists (rs_tgt (preg_of r)). split; eauto. econs.
+    - eapply Mem.loadv_inject in H0; des; eauto.
+      + esplits; eauto. econs; eauto.
+      + ss. specialize (AGREE RSP).
+        destruct (rs_src RSP); clarify.
+        inv AGREE; ss. econs; eauto.
+        rewrite Ptrofs.add_assoc. 
+        rewrite Ptrofs.add_assoc. f_equal.
+        apply Ptrofs.add_commut.
+  Qed.
+
+  Lemma extcall_arguments_inject sg j rs_src rs_tgt m_src m_tgt args_src 
+        (AGREE: agree j rs_src rs_tgt)
+        (INJECT: Mem.inject j m_src m_tgt)
+        (ARGS: extcall_arguments rs_src m_src sg args_src)
+    :
+      exists args_tgt,
+        extcall_arguments rs_tgt m_tgt sg args_tgt /\
+        Val.inject_list j args_src args_tgt.
+  Proof.
+    unfold extcall_arguments in *.
+    revert args_src ARGS. induction (loc_arguments sg); i; ss.
+    - inv ARGS. exists []. split; econs.
+    - inv ARGS. inv H1.
+      + eapply extcall_arg_inject in H; eauto. apply IHl in H3. des.
+        exists (v_tgt :: args_tgt). split.
+        * econs; eauto. econs; eauto.
+        * econs; eauto.
+      + eapply extcall_arg_inject in H; eauto.
+        eapply extcall_arg_inject in H0; eauto. apply IHl in H3. des.
+        exists (Val.longofwords v_tgt0 v_tgt :: args_tgt). split.
+        * econs; eauto. econs; eauto.
+        * econs; eauto. eapply Val.longofwords_inject; eauto.
+  Qed.
+
+  Lemma syscall_receptive
+        st_src0 st_src1 st_tgt0 args frs fptr tr0 n0
+        (STATE: st_src0 = Callstate args frs)
+        (FPTR: fptr = args.(Args.fptr))
+        (SYSMOD: ge.(Ge.find_fptr_owner)
+                      fptr (System.modsem skenv_link))
+        (MTCHST: match_states st_src0 st_tgt0 n0)
+        (STEP0: Sem.step ge st_src0 tr0 st_src1)
+    :
+      receptive_at (sem prog) st_src1.
+  Proof.
+    clarify. inv STEP0.
+    destruct (find_fptr_owner_determ SYSMOD MSFIND).
+    eapply system_receptive_at.
+  Qed.  
+
+  Lemma syscall_simulation
+        st_src0 st_src1 st_src2 st_tgt0 args frs fptr tr0 tr1 n0
+        (STATE: st_src0 = Callstate args frs)
+        (FPTR: fptr = args.(Args.fptr))
+        (SYSMOD: ge.(Ge.find_fptr_owner)
+                      fptr (System.modsem skenv_link))
+        (MTCHST: match_states st_src0 st_tgt0 n0)
+        (STEP0: Sem.step ge st_src0 tr0 st_src1)
+        (STEP1: Sem.step ge st_src1 tr1 st_src2)
+    :
+      receptive_at (sem prog) st_src2 /\
+      exists st_tgt1 n1,
+        (<< STEPTGT: Asm.step tge st_tgt0 tr1 st_tgt1 >>) /\
+        (<< MTCHST: forall st_src3 tr2
+                           (STEP2: Sem.step ge st_src2 tr2 st_src3),
+            match_states st_src3 st_tgt1 n1 /\ tr2 = E0>>) /\
+        (n1 < length frs + 3)%nat.
+  Proof.
+    clarify; inv MTCHST; inv STEP0; ss.
+    destruct (find_fptr_owner_determ SYSMOD MSFIND). ss. inv INIT.
+    inv STEP1; ss; [|inv FINAL]. inv STEP.    
+    exploit extcall_arguments_inject; eauto.
+    i. des.
+    exploit external_call_mem_inject_gen.
+    - eapply system_symbols_inject; eauto.
+    - eapply EXTCALL.
+    - eapply freed_from_inject; eauto.
+    - eauto.
+    - i. des.
+      unfold Frame.update_st. ss.
+      split.
+      { eapply system_receptive_at. }
+      exists (Asm.State
+                ((set_pair (loc_external_result (ef_sig ef)) vres'
+                      (regset_after_external rs_tgt)) #PC <- (rs_tgt RA))
+                m2').
+      inv STACK.
+      { exfalso. clarify.
+        rewrite FPTR in *.
+        unfold System.globalenv, initial_regset in *.
+        rewrite Pregmap.gso in FPTR0; [| intros EQ; inv EQ].
+        rewrite Pregmap.gso in FPTR0; [| intros EQ; inv EQ].
+        rewrite Pregmap.gss in FPTR0.
+        rewrite skenv_link_main in FPTR0. clarify.
+      }
+      assert (SIGEQ: SkEnv.get_sig skd = ef_sig ef).
+      { eapply external_function_sig; eauto. }
+      exists (
+        if
+          external_state (local_genv p)
+                         ((set_pair (loc_external_result (ef_sig ef)) (Retv.v retv)
+                                    (regset_after_external st.(st_rs))) # PC <- (st.(st_rs) RA) PC)
+        then (length frs0 + 2)%nat
+        else 0%nat).
+      splits.
+      + set (AGREEPC:= AGREE PC). rewrite <- FPTR in *.
+        destruct (Args.fptr args) eqn:EQ; ss; des_ifs; clarify. inv AGREEPC.       
+        econs 3.
+        * instantiate (1 := b2).
+          assert (delta = 0); clarify.
+          eapply system_function_ofs; eauto.
+        * instantiate (1 := ef).
+          eapply system_sig; eauto.
+        * instantiate (1 := args_tgt).
+          rewrite <- SIGEQ. auto.
+        * eapply H1.
+        * auto.
+      + i. inv STEP2; [inv AT|inv STEP|]. inv FINAL. split; auto.
+        ss. unfold Frame.update_st. ss. inv AFTER. ss. clarify.
+        assert (SGEQ: sg = ef_sig ef).
+        { des. rewrite FPTR in *. clarify. } clarify.
+        econs; cycle 3.
+        * ss.
+        * eapply match_stack_incr with (j2 := f'); eauto.
+        * ss.
+        * unfold set_pair. des_ifs; repeat (eapply update_agree2; eauto).
+          -- unfold regset_after_external.
+             intros []; des_ifs; try econs; eauto.
+          -- unfold regset_after_external.
+             intros []; des_ifs; try econs; eauto.
+          -- eapply Val.hiword_inject; eauto.
+          -- eapply Val.loword_inject; eauto.
+        * set (AGREE RSP). rewrite RSPPTR in *. clarify.
+          inv i.
+          eapply private_unfree_inj; eauto.          
+          { ii. rewrite Ptrofs.unsigned_zero in *.
+            exploit Mem.unchanged_on_perm; eauto.
+            - eapply freed_from_out_of_reach; eauto. rewrite SIGEQ. eauto.
+            - eapply Mem.mi_mappedblocks; eauto.
+            - intros PERM. eapply PERM.
+              exploit Mem.perm_inject; eauto.
+              eapply freed_from_perm; eauto. instantiate (1:=ofs-delta).
+              rewrite SIGEQ. omega.
+              i. replace ofs with (ofs - delta + delta); [auto|omega].
+          }
+          i. eapply separated_out_of_reach; cycle 2; eauto.          
+          -- eapply Mem.mi_mappedblocks; eauto.
+          -- eapply freed_from_out_of_reach; eauto.
+             rewrite Ptrofs.unsigned_zero in *. rewrite SIGEQ. omega.
+          -- i. eapply ec_max_perm; eauto. eapply external_call_spec.
+          -- eapply freed_from_inject; eauto.
+        * etrans; eauto.
+      + ss. des_ifs; omega.
+  Qed.
+
+  Lemma match_states_call_ord_1 args frs st_tgt n
+        (MTCHST: match_states (Callstate args frs) st_tgt n)
+    :
+      1%nat = n.
+  Proof. inv MTCHST. auto. Qed.
+
+  Lemma src_receptive_at st_src st_tgt n
+        (MTCHST: match_states st_src st_tgt n)
+    :
+      receptive_at (sem prog) st_src.
+  Proof.
+  Admitted.
+
+  Lemma match_state_xsim
+    :
+      forall st_src st_tgt n (MTCHST: match_states st_src st_tgt n),
+        xsim (sem prog) (semantics tprog) lt n st_src st_tgt.
+  Proof.
+    pcofix CIH. i. pfold. destruct st_src.
+    - exploit init_case; ss.
+      instantiate (1:=frs). instantiate (2:=args). i. des.
+      + destruct (match_states_call_ord_1 MTCHST).
+        right. econs; i.
+        * exfalso. inv MTCHST. inv FINALTGT. inv ASMMOD.
+          inv MSFIND. unfold Genv.find_funct in *. des_ifs.
+          specialize (AGREE PC). rewrite <- FPTR in *.
+          inv AGREE. unfold Vnullptr in *. des_ifs. congruence.
+        * exploit step_init_simulation; try eassumption.
+          i. des. econs 2; ss; eauto. rewrite LINK_SK.
+          split; auto. apply star_one. eauto.
+      + left. econs.
+        { i. exfalso. inv FINALSRC. }
+        econs; [|eapply src_receptive_at; eauto].
+        i.
+        destruct (call_step_noevent STEPSRC).
+        destruct (match_states_call_ord_1 MTCHST).
+        exists 0%nat. exists st_tgt. split.
+        { right. split; [apply star_refl|omega]. }
+        left. pfold. left.
+        econs.
+        { i. exfalso. inv STEPSRC. ss. rewrite LINK_SK in *.
+          destruct (find_fptr_owner_determ SYSMOD MSFIND).
+          inv INIT. inv FINALSRC. inv FINAL.
+        }
+        econs; cycle 1.
+        { inv STEPSRC. ss. rewrite LINK_SK in *.
+          destruct (find_fptr_owner_determ SYSMOD MSFIND). ss.
+          eapply system_receptive_at.
+        }
+        i. exists (length frs + 3)%nat. ss. rewrite LINK_SK in *.
+        exploit syscall_simulation; eauto.
+        i. des. exists st_tgt1. split.
+        { left. apply plus_one. econs; [apply asm_determinate_at|]. auto. }
+        left. pfold. left.
+        econs.
+        { i. exfalso. inv STEPSRC. ss.
+          destruct (find_fptr_owner_determ SYSMOD MSFIND).
+          inv INIT. inv STEPSRC0; ss; [|inv FINAL].
+          inv STEP. inv FINALSRC. ss. inv MTCHST.
+          inv STACK. inv SYSMOD. ss.
+          exploit system_genv_skenv; eauto. i. clarify.
+        }
+        econs; auto.
+        i.
+        ss. rewrite LINK_SK in *. apply MTCHST0 in STEPSRC1. des. clarify.
+        exists n1, st_tgt1. split.
+        { right. split; auto. apply star_refl. }
+        right. eauto.
+      + right. econs; i; try (exfalso; eauto).          
+    - left. econs.
+      + i. econs.
+        * exploit transf_final_states; eauto.
+        * i. inv FINAL0. inv FINAL1. eq_closure_tac.
+        * ii. inv FINAL. inv H; eq_closure_tac.
+      + econs.
+        * i. ss. rewrite LINK_SK in *.
+          exploit normal_state_fsim_step; eauto.
+          i. des; esplits; eauto.
+          -- left. econs; ss.
+             ++ econs; eauto.
+                apply asm_determinate_at.
+             ++ econs 1.
+             ++ rewrite E0_right. auto.
+          -- right. econs; ss. clarify. econs.
+        * eapply src_receptive_at; eauto.
+  Qed.
+
+  Lemma transf_xsim_properties
+    :
+        xsim_properties (sem prog) (semantics tprog) nat lt.
+  Proof.
+    econs; [apply lt_wf| |apply symb_preserved].
+    econs. i.
+    exploit (transf_initial_states); eauto.
+    i. des. esplits. econs; eauto.
+    - i. inv INIT0. inv INIT1. clarify.
+    - apply match_state_xsim; eauto.
+  Qed.
+
+  Lemma transf_program_correct:
+    mixed_simulation (Sem.sem prog) (Asm.semantics tprog).
+  Proof.
+    eapply Mixed_simulation. eapply transf_xsim_properties.
+  Qed.    
+
+End PRESERVATION.
