x86/SimMemExtends.v
@@ -1,0 +1,101 @@
+Require Import CoqlibC.
+Require Import Memory.
+Require Import Values.
+Require Import Maps.
+Require Import Events.
+Require Import Globalenvs.
+Require Import sflib.
+Require Import RelationClasses.
+Require Import FSets.
+Require Import Ordered.
+Require Import AST.
+Require Import Integers.
+
+Require Import IntegersC LinkingC.
+Require Import SimSymb Skeleton Mod ModSem.
+Require SimSymbId.
+Require Import SimMem.
+
+Set Implicit Arguments.
+
+
+
+
+Record t' := mk {
+  src: mem;
+  tgt: mem;
+}.
+
+Program Instance SimMemExtends : SimMem.class :=
+{
+  t := t';
+  src := src;
+  tgt := tgt;
+  wf := fun (rel: t') => Mem.extends rel.(src) rel.(tgt);
+  le := fun (mrel0 mrel1: t') => True;
+  lift := id;
+  unlift := fun _ => id;
+  sim_val := fun (_: t') => Val.lessdef;
+  sim_val_list := fun (_: t') => Val.lessdef_list;
+}.
+Next Obligation.
+  ss.
+Qed.
+Next Obligation.
+  do 2 (apply Axioms.functional_extensionality; i).
+  apply prop_ext.
+  split; i; ss; clarify.
+  - ginduction x; ii; inv H; ss.
+    econs; eauto.
+  - induction H; econs; eauto.
+Qed.
+
+Global Program Instance SimSymbExtends: SimSymb.class SimMemExtends := {
+  t := unit;
+  le := SimSymbId.le;
+  sim_sk := SimSymbId.sim_sk;
+  sim_skenv (_: SimMem.t) (_: unit) := SimSymbId.sim_skenv;
+}
+.
+Next Obligation.
+  ss.
+Qed.
+Next Obligation.
+  eapply SimSymbId.sim_sk_link; eauto.
+Qed.
+Next Obligation.
+  exploit SimSymbId.sim_sk_load_sim_skenv; eauto. i; des.
+  eexists. eexists (mk _ _).
+  esplits; ss; eauto.
+  apply Mem.extends_refl.
+Qed.
+Next Obligation.
+  eapply SimSymbId.sim_skenv_monotone; try apply SIMSKENV; eauto.
+Qed.
+Next Obligation.
+  exploit SimSymbId.sim_skenv_func_bisim; eauto.
+  i; des.
+  inv H. inv SIMSKENV.
+  econs; eauto.
+  - ii; ss.
+    eapply FUNCFSIM; eauto.
+    rpapply FUNCSRC. f_equal.
+    inv SIMFPTR; ss.
+  - ii; ss.
+    eapply FUNCBSIM; eauto.
+    rpapply FUNCTGT. f_equal.
+    inv SIMFPTR; ss.
+Qed.
+Next Obligation.
+  esplits; eauto.
+  eapply SimSymbId.system_sim_skenv; eauto.
+Qed.
+Next Obligation.
+  inv ARGS; ss. destruct args_src, args_tgt; destruct sm0; ss; clarify.
+  exploit external_call_mem_extends; eauto. i. des. 
+  exists (mk retv_src.(Retv.m) m2'). exists (Retv.mk vres' m2').
+  esplits; ss; eauto.
+  eapply external_call_symbols_preserved; eauto.
+  eapply SimSymbId.sim_skenv_equiv; eauto.
+Qed.
+
